Make ssimpl handle lpropand
We now look through the list of hypotheses, and remove any conclusion
that matches.  We do not strip propositions from the hypotheses, and
instead introduce them into the Coq context.  Because we used to look
through the conclusions rather than the hypotheses, I strengthened
lentails to lequiv, and automated the proofs that required non-trivial
tweaking to deal with this change.

Hopefully most of the timing diff is just system noise.

After     | File Name               | Before    || Change
------------------------------------------------------------
19m28.57s | Total                   | 18m33.26s || +0m55.30s
------------------------------------------------------------
0m12.74s  | septac                  | 0m06.83s  || +0m05.91s
0m33.63s  | x86/cfuncspec           | 0m30.16s  || +0m03.47s
0m32.00s  | x86/screenproof         | 0m28.13s  || +0m03.87s
0m29.60s  | x86/listproof           | 0m25.76s  || +0m03.83s
0m21.43s  | x86/wrapalloc           | 0m18.43s  || +0m03.00s
0m19.75s  | x86/programassemcorrect | 0m17.12s  || +0m02.62s
0m53.52s  | x86/instrrules/addsub   | 0m52.25s  || +0m01.27s
0m34.53s  | x86/instrrules/cmp      | 0m33.35s  || +0m01.17s
0m28.58s  | x86/imp                 | 0m27.55s  || +0m01.02s
0m28.33s  | x86/lifeimp             | 0m27.11s  || +0m01.21s
0m25.82s  | x86/instrrules/and      | 0m24.56s  || +0m01.26s
0m24.46s  | x86/instrrules/adc      | 0m23.38s  || +0m01.08s
0m21.94s  | x86/instrcodec          | 0m20.62s  || +0m01.32s
0m19.50s  | pointsto                | 0m17.62s  || +0m01.87s
0m14.22s  | x86/win/pecoff          | 0m12.45s  || +0m01.77s
0m10.86s  | codec                   | 0m09.06s  || +0m01.79s
0m07.96s  | spred                   | 0m06.42s  || +0m01.54s
0m07.95s  | obs                     | 0m06.29s  || +0m01.66s
0m07.72s  | triple/roc              | 0m06.59s  || +0m01.12s
0m07.50s  | x86/program             | 0m06.43s  || +0m01.07s
0m01.87s  | charge_lemmas           |    N/A    || +0m01.87s
0m37.37s  | examples/mulc           | 0m36.78s  || +0m00.58s
0m31.25s  | examples/specexamples   | 0m31.06s  || +0m00.19s
0m29.28s  | triple/set              | 0m28.54s  || +0m00.74s
0m27.64s  | x86/macros              | 0m27.05s  || +0m00.58s
0m24.03s  | x86/instrrules/shift    | 0m24.84s  || -0m00.80s
0m19.49s  | x86/inlinealloc         | 0m19.41s  || +0m00.07s
0m19.03s  | x86/instrrules/callrel  | 0m19.58s  || -0m00.54s
0m18.92s  | x86/instrrules/incdec   | 0m18.63s  || +0m00.29s
0m18.55s  | x86/instrrules/mov      | 0m18.38s  || +0m00.17s
0m17.38s  | x86/instrrules/jmprel   | 0m17.12s  || +0m00.25s
0m17.30s  | x86/main                | 0m17.90s  || -0m00.59s
0m17.19s  | x86/call                | 0m17.30s  || -0m00.10s
0m15.94s  | bitstest                | 0m15.08s  || +0m00.85s
0m14.21s  | bitsopsprops            | 0m14.20s  || +0m00.01s
0m13.94s  | spec                    | 0m13.32s  || +0m00.61s
0m12.81s  | x86/instrrules/core     | 0m12.87s  || -0m00.05s
0m11.20s  | x86/instrrules/push     | 0m11.39s  || -0m00.19s
0m10.95s  | x86/instrrules/pop      | 0m10.98s  || -0m00.03s
0m10.90s  | examples/xorswap        | 0m10.30s  || +0m00.59s
0m10.46s  | x86/cstringimp          | 0m10.84s  || -0m00.37s
0m10.42s  | spectac                 | 0m09.64s  || +0m00.77s
0m09.44s  | x86/instrrules/xor      | 0m10.24s  || -0m00.80s
0m08.65s  | x86/gcdex               | 0m08.34s  || +0m00.31s
0m08.41s  | x86/instrrules/not      | 0m08.05s  || +0m00.35s
0m08.34s  | triple/get              | 0m07.94s  || +0m00.39s
0m08.19s  | x86/instrrules/or       | 0m08.06s  || +0m00.12s
0m08.11s  | x86/instrrules/neg      | 0m07.75s  || +0m00.35s
0m07.97s  | x86/basic               | 0m07.94s  || +0m00.02s
0m07.81s  | x86/basicprog           | 0m07.22s  || +0m00.58s
0m07.35s  | opred/laws              | 0m07.69s  || -0m00.34s
0m07.29s  | x86/instrrules/jccrel   | 0m07.30s  || -0m00.00s
0m06.81s  | examples/fact           | 0m06.77s  || +0m00.04s
0m06.54s  | triple/morphisms        | 0m05.78s  || +0m00.75s
0m06.37s  | x86/step                | 0m05.71s  || +0m00.66s
0m06.33s  | x86/instrrules/test     | 0m06.70s  || -0m00.37s
0m06.22s  | x86/screenimp           | 0m06.63s  || -0m00.41s
0m06.17s  | examples/entry          | 0m06.26s  || -0m00.08s
0m06.16s  | x86/instrrules/ret      | 0m06.55s  || -0m00.38s
0m06.16s  | triple/read             | 0m05.39s  || +0m00.77s
0m06.15s  | roundtrip               | 0m05.85s  || +0m00.30s
0m06.03s  | x86/listspec            | 0m06.33s  || -0m00.29s
0m06.02s  | x86/testrun             | 0m05.86s  || +0m00.15s
0m05.92s  | x86/listimp             | 0m06.26s  || -0m00.33s
0m05.88s  | x86/examples            | 0m05.69s  || +0m00.18s
0m05.88s  | x86/instrrules/in       | 0m06.10s  || -0m00.21s
0m05.83s  | x86/cfunc               | 0m05.99s  || -0m00.16s
0m05.81s  | x86/instrrules/lea      | 0m06.10s  || -0m00.29s
0m05.78s  | safe                    | 0m05.31s  || +0m00.47s
0m05.65s  | triple/seplogic         | 0m05.47s  || +0m00.18s
0m05.63s  | triple/monad            | 0m05.33s  || +0m00.29s
0m05.61s  | x86/instrrules/out      | 0m05.93s  || -0m00.31s
0m05.57s  | chargetac               | 0m04.62s  || +0m00.95s
0m05.54s  | basicspectac            | 0m05.64s  || -0m00.09s
0m05.44s  | codecregex              | 0m05.35s  || +0m00.09s
0m05.38s  | triple/get_readable     | 0m05.11s  || +0m00.26s
0m05.32s  | bitreader               | 0m05.03s  || +0m00.29s
0m05.23s  | x86/screenspec          | 0m05.20s  || +0m00.03s
0m05.10s  | triple/tactics          | 0m04.67s  || +0m00.42s
0m05.00s  | x86/programeq           | 0m05.00s  || +0m00.00s
0m04.99s  | spredtotal              | 0m04.02s  || +0m00.97s
0m04.91s  | x86/instrrules          | 0m05.00s  || -0m00.08s
0m04.90s  | triple/core             | 0m04.62s  || +0m00.28s
0m04.90s  | x86/programassem        | 0m04.86s  || +0m00.04s
0m04.66s  | cursor                  | 0m04.50s  || +0m00.16s
0m04.45s  | x86/procstate           | 0m03.82s  || +0m00.63s
0m04.35s  | x86/procstatemonad      | 0m03.56s  || +0m00.78s
0m04.32s  | x86/mem                 | 0m03.85s  || +0m00.47s
0m04.28s  | x86/eval                | 0m03.82s  || +0m00.46s
0m04.27s  | writer                  | 0m04.06s  || +0m00.20s
0m04.27s  | opred                   | 0m03.96s  || +0m00.30s
0m04.18s  | bitscodec               | 0m04.10s  || +0m00.08s
0m04.08s  | triple                  | 0m04.04s  || +0m00.04s
0m04.06s  | opred/pointed           | 0m04.08s  || -0m00.02s
0m03.94s  | reader                  | 0m03.68s  || +0m00.25s
0m03.90s  | opred/morphisms         | 0m03.90s  || +0m00.00s
0m03.43s  | x86/instrsyntax         | 0m03.49s  || -0m00.06s
0m03.32s  | x86/flags               | 0m03.40s  || -0m00.08s
0m03.27s  | x86/ioaction            | 0m03.25s  || +0m00.02s
0m03.08s  | opred/core              | 0m03.00s  || +0m00.08s
0m02.93s  | bitsops                 | 0m02.90s  || +0m00.03s
0m02.80s  | monadinst               | 0m02.91s  || -0m00.11s
0m01.60s  | common_tactics          | 0m01.56s  || +0m00.04s
0m00.42s  | common_definitions      | 0m00.40s  || +0m00.01s

src/septac.v
@@ -1,6 +1,7 @@
 Require Import Ssreflect.ssreflect Ssreflect.ssrbool Ssreflect.ssrnat Ssreflect.ssrfun Ssreflect.eqtype Ssreflect.seq.
 Require Import x86proved.spred.
-Require Import x86proved.common_tactics.
+Require Import x86proved.common_tactics x86proved.charge_lemmas.
+Require Import Coq.Classes.RelationClasses.
 
 Set Implicit Arguments.
 Unset Strict Implicit.
@@ -233,40 +234,66 @@ Module Solving.
 
     Lemma eqn'P i j : reflect (i = j) (eqn' i j).
     Proof. apply eqnP. Qed.
+
+    Definition LOOKUP_FAILURE {T} {x : T} := x.
   End Indexes.
 
   Inductive term :=
   | t_atom (i: idx)
   | t_star (t1 t2: term)
+  | t_propand (i: idx) (t: term)
   | t_emp
   | t_false.
 
   (* Idea: reflect lhs first and choose index for each rhs term with a hole to
      be the first lhs atom that unifies. *)
 
-  Definition alist := seq (idx * SPred).
-  Definition env := (idx * alist)%type.
+  Definition spred_alist := seq (idx * SPred).
+  Definition prop_alist := seq (idx * Prop).
+  Definition env := (idx * spred_alist * prop_alist)%type.
 
-  Fixpoint lookup (a: alist) (i: idx) : SPred :=
+  Fixpoint spred_lookup (a: spred_alist) (i: idx) : SPred :=
     match a with
-    | (j,P) :: a' => if eqn' i j then P else lookup a' i
-    | [::] => empSP (* default value; shouldn't happen *)
+    | (j,P) :: a' => if eqn' i j then P else spred_lookup a' i
+    | [::] => @LOOKUP_FAILURE _ empSP (* default value; shouldn't happen *)
+    end.
+
+  Fixpoint prop_lookup (a: prop_alist) (i: idx) : Prop :=
+    match a with
+    | (j,P) :: a' => if eqn' i j then P else prop_lookup a' i
+    | [::] => @LOOKUP_FAILURE _ False (* default value; shouldn't happen *)
     end.
 
   Fixpoint eval (e: env) (t: term) : SPred :=
     match t with
-    | t_atom i => let (_, a) := e in lookup a i
+    | t_atom i => let: (_, a, _) := e in spred_lookup a i
     | t_star t1 t2 => eval e t1 ** eval e t2
+    | t_propand i t => (let: (_, _, a) := e in prop_lookup a i) /\\ eval e t
     | t_emp => empSP
     | t_false => lfalse
     end.
 
   (* Inserts an SPred into an environment. Calls its continuation with the
      updated environment and the index where the predicate was inserted. *)
-  Ltac insert_tac e(*:env*) P(*:SPred*) cont(*: env -> idx -> tactic *) :=
+  Definition spred_insert (e: env) (P: SPred) : env * idx :=
     match e with
-    | (?i, ?a) => cont (i.+1, (i,P)::a) i
+      | (i, a, a') => ((i.+1, (i,P)::a, a'), i)
     end.
+  Ltac spred_insert_tac e(*:env*) P(*:SPred*) cont(*: env -> idx -> tactic *) :=
+    let e'i := constr:(spred_insert e P) in
+    let e' := (eval hnf in e'i.1) in
+    let i := (eval hnf in e'i.2) in
+    cont e' i.
+
+  Definition prop_insert (e: env) (P: Prop) : env * idx :=
+    match e with
+      | (i, a, a') => ((i.+1, a, (i,P)::a'), i)
+    end.
+  Ltac prop_insert_tac e(*:env*) P(*:Prop*) cont(*: env -> idx -> tactic *) :=
+    let e'i := constr:(prop_insert e P) in
+    let e' := (eval hnf in e'i.1) in
+    let i := (eval hnf in e'i.2) in
+    cont e' i.
 
   (* Quote left-hand side of entailment. Duplicated terms don't get to share
      indices since this should not typically happen. *)
@@ -274,27 +301,32 @@ Module Solving.
      "returns" both an updated environment and a quoted term. Ltac doesn't make
      it easy to return tuples, but CPS is easy. *)
   Ltac lquote e(*:env*) P(*:SPred*) cont(*: env -> term -> tactic *) :=
-    match P with
+    idtac;
+    lazymatch P with
     | ?P1 ** ?P2 =>
         lquote e P1 ltac:(fun e t1 =>
         lquote e P2 ltac:(fun e t2 =>
         cont e (t_star t1 t2)))
+    | ?P /\\ ?T
+      => prop_insert_tac e P ltac:(fun e p =>
+         lquote e T ltac:(fun e t =>
+         cont e (t_propand p t)))
     | lfalse => cont e t_false
     | empSP => cont e t_emp
-    | _ => insert_tac e P ltac:(fun e i => cont e (t_atom i))
+    | _ => spred_insert_tac e P ltac:(fun e i => cont e (t_atom i))
     end.
 
   (*
   Goal forall P: SPred, True.
     move=> P.
-    lquote ((0, [::]) : env) (P ** empSP ** P ** lprop (0 + 0 = 0)) ltac:(fun e t =>
+    lquote ((0, [::], [::]) : env) (P ** empSP ** P ** lpropand (0 + 0 = 0) empSP) ltac:(fun e t =>
       idtac e; idtac t;
-      let P := eval cbv [eval lookup eqn'] in (eval e t) in idtac P
+      let P := eval cbv [eval spred_lookup prop_lookup eqn'] in (eval e t) in idtac P
     ).
     apply I. Qed.
   *)
 
-  (* Succeed iff t fails *)
+  (* Succeed iff t fails or completely solves the goal *)
   Tactic Notation "not" tactic1(t) := try (t; fail 1).
 
   (* This tactic succeeds if its two arguments are equal modulo alpha conversion
@@ -317,7 +349,7 @@ Module Solving.
      inside P and a. *)
   Ltac lookup_tac doUnify a(*:alist*) P(*:SPred*)
       found(*: idx -> tactic*) notfound(*: unit -> tactic*) :=
-    match a with
+    match eval hnf in a with
     | (?i, ?P') :: _ =>
       (* We don't unify with something that's entirely an evar. This would lead
          to very random behaviour. *)
@@ -333,31 +365,39 @@ Module Solving.
      the [unify] tactic (https://github.com/coq/coq/commit/18e6108339aaf18499).
    *)
   Ltac rquote doUnify e(*:env*) P(*:SPred*) cont(*: env -> term -> tactic *) :=
-    match P with
+    idtac;
+    lazymatch P with
     | ?P1 ** ?P2 =>
         rquote doUnify e P1 ltac:(fun e t1 =>
         rquote doUnify e P2 ltac:(fun e t2 =>
         cont e (t_star t1 t2)))
+    | ?P /\\ ?T =>
+        rquote doUnify e T ltac:(fun e t =>
+          let a' := match e with (_, ?a, ?a') => constr:(a') end in
+          lookup_tac doUnify a' P
+            ltac:(fun j => cont e (t_propand j t))
+            ltac:(fun _ => prop_insert_tac e P ltac:(fun e i => cont e (t_propand i t))))
     | empSP => cont e t_emp
     | lfalse => cont e t_false
     | ltrue =>
           (* We don't match up ltrue. We leave it untouched on the right-hand
              side and let the user decide what to do with it. *)
-           insert_tac e P ltac:(fun e i => cont e (t_atom i))
-    | ?dummy_name => is_evar P;
-          (* If an atom is entirely an evar, we don't touch it. Otherwise, it
-             would unify with the first thing it saw on the left, which is
-             probably not what the user expects. *)
-           insert_tac e P ltac:(fun e i => cont e (t_atom i))
-    | _ =>
-        match e with
-        | (_, ?a) =>
-          lookup_tac doUnify a P
-            ltac:(fun j => cont e (t_atom j))
-            ltac:(fun _ => insert_tac e P ltac:(fun e i => cont e (t_atom i)))
-        end
+           spred_insert_tac e P ltac:(fun e i => cont e (t_atom i))
+    | _ => first [ is_evar P;
+                   (* If an atom is entirely an evar, we don't touch it. Otherwise, it
+                      would unify with the first thing it saw on the left, which is
+                      probably not what the user expects. *)
+                   spred_insert_tac e P ltac:(fun e i => cont e (t_atom i))
+                 | idtac;
+                   match e with
+                     | (_, ?a, ?a') =>
+                       lookup_tac doUnify a P
+                         ltac:(fun j => cont e (t_atom j))
+                         ltac:(fun _ => spred_insert_tac e P ltac:(fun e i => cont e (t_atom i)))
+                   end ]
     end.
 
+  (** Remove one instance of the atom with index [i] *)
   Fixpoint remove_atom t i : option term :=
     match t with
     | t_atom i' => if eqn' i' i then Some t_emp else None
@@ -370,10 +410,37 @@ Module Solving.
             | None => None
             end
         end
+    | t_propand P t' =>
+      match remove_atom t' i with
+        | Some t'' => Some (t_propand P t'')
+        | None => None
+      end
     | t_emp => None
     | t_false => None
     end.
 
+  (** Remove all instances of the prop with index [i] *)
+  Fixpoint remove_prop t i : option term :=
+    match t with
+    | t_atom i' => None
+    | t_star t1 t2 =>
+        match remove_prop t1 i, remove_prop t2 i with
+        | Some t1', Some t2' => Some (t_star t1' t2')
+        | Some t1', None => Some (t_star t1' t2)
+        | None, Some t2' => Some (t_star t1 t2')
+        | None, None => None
+        end
+    | t_propand p t' => if eqn' p i
+                        then match remove_prop t' i with
+                               | Some t'' => Some t''
+                               | None => Some t'
+                             end
+                        else None
+    | t_emp => None
+    | t_false => None
+    end.
+
+  (** Remove all terms showing up in [tQ] from [tP]. *)
   Fixpoint remove (tP tQ: term) : option term :=
     match tQ with
     | t_atom i => remove_atom tP i
@@ -382,101 +449,192 @@ Module Solving.
         | Some tP' => remove tP' t2
         | None => None
         end
+    | t_propand P t =>
+        match remove tP t with
+        | Some tP' => remove_prop tP' P
+        | None => None
+        end
     | t_emp => Some tP
     | t_false => None
     end.
 
+  Local Ltac cancel_sepSP :=
+    idtac;
+    match goal with
+      | [ |- ?a ** ?b |-- ?a ** ?b' ] => (f_cancel; [])
+      | [ |- ?a ** ?b |-- ?a' ** ?b ] => (f_cancel; [])
+      | [ |- ?a ** ?b -|- ?a ** ?b' ] => (f_cancel; [])
+      | [ |- ?a ** ?b -|- ?a' ** ?b ] => (f_cancel; [])
+    end.
+
+  Local Ltac t_septac' :=
+    idtac;
+    match goal with
+      | _ => reflexivity
+      | _ => eassumption
+      | _ => progress simpl_paths
+      | _ => progress subst
+      | _ => progress simpl
+      | _ => progress rewrite ?eq_refl ?empSPL ?empSPR ?sepSPA
+      | _ => progress setoid_rewrite <- bilpropandL
+      | _ => progress setoid_rewrite <- bilpropandR
+      | _ => rewrite ?sepSPA; progress cancel_sepSP
+      | _ => rewrite -?sepSPA; progress cancel_sepSP
+      | _ => progress destruct_head ex
+      | _ => progress destruct_head and
+      | [ H : eval _ _ -|- _ |- _ ] => setoid_rewrite -> H; clear H
+      | [ H : context[?a == ?a] |- _ ] => rewrite eq_refl in H
+      | [ H : context[eqn' ?a ?b] |- _ ] => change (eqn' a b) with (a == b) in *; case_eq (a == b) => *
+      | [ H : (?a == ?b) = _, H' : context[?a == ?b] |- _ ] => rewrite H in H'
+      | [ H : (?a == ?b) = true |- _ ] => move/eqP in H
+      | [ |- _ /\\ _ |-- _ ] => apply lpropandL => *
+      | [ |- _ |-- _ /\\ _ ] => (apply lpropandR; try assumption)
+      | [ H : forall _, Some _ = Some _ -> _ |- _ ] => specialize (H _ (reflexivity _))
+      | [ H : forall _, None = Some _ -> _ |- _ ] => clear H
+      | [ H : forall _ _, (_, _) = (_, _) -> _ |- _ ] => specialize (H _ _ (reflexivity _))
+      | [ |- ?a ** ?b -|- ?b ** ?a ] => by rewrite sepSPC
+      | [ |- _ /\\ _ |-- _ ] => apply lpropandL => *
+      | [ |- _ |-- _ /\\ _ ] => (apply lpropandR; first by eassumption)
+    end.
+
+  Local Ltac t_remove' :=
+    idtac;
+    match goal with
+      | _ => t_septac'
+      | [ H : context[match remove_prop ?a ?b with _ => _ end] |- _ ]
+        => (destruct (remove_prop a b); try done)
+      | [ H : context[remove_atom ?a ?b] |- _ ]
+        => (destruct (remove_atom a b); try done)
+    end.
+
+  Local Ltac t_remove := do ?[ t_remove' | split; by t_remove ].
+
   Lemma remove_atom_correct e t i tR:
     remove_atom t i = Some tR ->
-    eval e t |-- eval e (t_atom i) ** eval e tR.
+    eval e t -|- eval e (t_atom i) ** eval e tR.
   Proof.
-    move: tR. elim: t; try done.
-    - move=> i' tR /=. case: eqn'P => // [->] [<-].
-      by rewrite empSPR.
-    - move=> t1 IHt1 t2 IHt2 tR /=.
-      destruct (remove_atom t1 i) as [t1'|].
-      - move=> [<-]. rewrite ->IHt1; last reflexivity. rewrite sepSPA.
-        reflexivity.
-      destruct (remove_atom t2 i) as [t1'|]; last done.
-      move=> [<-]. rewrite ->IHt2; last reflexivity.
-      rewrite -sepSPA [_ ** eval e (t_atom i)]sepSPC sepSPA. reflexivity.
+    move: tR.
+    (elim: t => /= *; try done);
+      t_remove.
+  Qed.
+
+  Lemma remove_prop_correct e t i tR:
+    remove_prop t i = Some tR ->
+    eval e t -|- eval e (t_propand i tR).
+  Proof.
+    move: tR.
+    (elim: t => /= *; try done);
+      t_remove.
   Qed.
 
   Lemma remove_correct e tP tQ tR:
     remove tP tQ = Some tR ->
-    eval e tP |-- eval e tQ ** eval e tR.
+    eval e tP -|- eval e tQ ** eval e tR.
   Proof.
     move: tP tR. elim: tQ.
-      move=> i tP tR /= HtR. exact: remove_atom_correct.
-
-      move=> t1 IHt1 t2 IHt2 tP tR /=.
+    { move=> i tP tR /= HtR. exact: remove_atom_correct. }
+    { move=> t1 IHt1 t2 IHt2 tP tR /=.
       specialize (IHt1 tP).
       destruct (remove tP t1) as [tP'|]; last done.
       move=> HtR. move/(_ _ _ HtR): IHt2 => Ht2.
-      rewrite sepSPA. rewrite <-Ht2. exact: IHt1.
+      rewrite sepSPA. rewrite <-Ht2. exact: IHt1. }
+    { move => /= i t IH tP *.
+      specialize (IH tP).
+      destruct (remove tP t); last by exfalso.
+      rewrite -> IH; clear IH; last by reflexivity.
+      let H := match goal with | [ H : remove_prop ?a ?b = Some _ |- _ ] => constr:(H) end in
+      rewrite -> (@remove_prop_correct _ _ _ _ H).
+      by do ![ progress simpl
+             | progress setoid_rewrite <- bilpropandL
+             | progress setoid_rewrite <- bilpropandR ]. }
 
-      move=> tP tR /= [<-]. by rewrite empSPL.
+    { move=> tP tR /= [<-]. by rewrite empSPL. }
 
-      move=> tP tR /=. done.
+    { move=> tP tR /=. done. }
   Qed.
 
-  Fixpoint simplify (tP tQ: term) : (term * term) :=
-    match tQ with
+  (** We have the option to remove matched [Prop] bits from the
+      hypotheses; we choose not to do so.  We treat [tH] as the
+      hypotheses and [tC] as the conclusions. *)
+  Fixpoint simplify (tC tH: term) : (term * term) :=
+    match tH with
     | t_atom i =>
-        match remove_atom tP i with
-        | Some tP' => (tP', t_emp)
-        | None => (tP, tQ)
+        match remove_atom tC i with
+        | Some tC' => (tC', t_emp)
+        | None => (tC, tH)
         end
     | t_star t1 t2 =>
-        let (tP', t1')  := simplify tP t1 in
-        let (tP'', t2') := simplify tP' t2 in
-        (tP'', t_star t1' t2')
-    | t_emp => (tP, tQ)
-    | t_false => (tP, tQ)
+        let (tC', t1')  := simplify tC t1 in
+        let (tC'', t2') := simplify tC' t2 in
+        (tC'', t_star t1' t2')
+    | t_propand P t =>
+        let (tC', t') := eta_expand (simplify tC t) in
+        match remove_prop tC' P with
+          | Some tC'' => (tC'', t_propand P t')
+          | None => (tC', t_propand P t')
+        end
+    | t_emp => (tC, tH)
+    | t_false => (tC, tH)
     end.
 
+  Local Ltac t_simplify_correct' :=
+    idtac;
+    match goal with
+      | [ e : env, H : context[match remove_atom ?a ?b with _ => _ end] |- _ ]
+        => pose proof (@remove_atom_correct e a b); destruct (remove_atom a b)
+      | [ e : env, H : context[match remove_prop ?a ?b with _ => _ end] |- _ ]
+        => pose proof (@remove_prop_correct e a b); destruct (remove_prop a b)
+      | _ => t_septac'
+    end.
+
+  Local Ltac t_simplify_correct :=
+    do ![ t_simplify_correct'
+        | eexists (t_propand _ _); by t_simplify_correct
+        | eexists (t_star _ _); by t_simplify_correct
+        | eexists (t_atom _); by t_simplify_correct
+        | exists t_emp; by t_simplify_correct
+        | eexists; by t_simplify_correct
+        | split; by t_simplify_correct ].
+
   (* Correctness theorem strong enough for induction. *)
-  (* This theorem could probably be strengthened to biimplication if that
-     seems useful at some point. *)
-  Lemma simplify_correct e tP tQ tP' tQ' :
-    simplify tP tQ = (tP', tQ') -> exists tR,
-    (eval e tP |-- eval e tP' ** eval e tR)  /\
-    (eval e tQ' ** eval e tR |-- eval e tQ).
+  Lemma simplify_correct e tH tC tH' tC' :
+    simplify tC tH = (tC', tH') -> exists tR,
+    (eval e tH -|- eval e tH' ** eval e tR)  /\
+    (eval e tC -|- eval e tC' ** eval e tR).
   Proof.
-    move: tP tP' tQ'. elim: tQ.
-    - move=> i tP tP' tQ' /=.
-      have Hatom := @remove_atom_correct e tP i.
-      destruct (remove_atom tP i).
-      - move=> [<- <-]. exists (t_atom i). rewrite ->Hatom; last reflexivity.
-        rewrite empSPL. split; last reflexivity. by rewrite sepSPC.
-      - move=> [<- <-]. exists t_emp. rewrite !empSPR. split; reflexivity.
-    - move=> t1 IHt1 t2 IHt2 tP tP'' tQ' /=.
-      specialize (IHt1 tP). destruct (simplify tP t1) as [tP' t1'].
-      specialize (IHt2 tP'). destruct (simplify tP' t2) as [ttmp t2'].
+    move: tC tC' tH'.
+    elim: tH.
+    { move => /= *; t_simplify_correct. }
+    { move=> t1 IHt1 t2 IHt2 tC tC'' tH' /=.
+      specialize (IHt1 tC). destruct (simplify tC t1) as [tC' t1'].
+      specialize (IHt2 tC'). destruct (simplify tC' t2) as [ttmp t2'].
       move=> [Htmp <-] /=. subst ttmp.
       edestruct IHt1 as [tR1 [Hpre1 Hpost1]]; first reflexivity.
       edestruct IHt2 as [tR2 [Hpre2 Hpost2]]; first reflexivity.
-      clear IHt1 IHt2. exists (t_star tR1 tR2) => /=. split.
-      - rewrite ->Hpre1, Hpre2. by rewrite sepSPA [eval e tR2 ** _]sepSPC.
-      - rewrite <-Hpost1. rewrite <-Hpost2. rewrite -sepSPA.
-        rewrite [_ ** eval e tR1]sepSPA [_ ** eval e tR1]sepSPC.
-        by rewrite !sepSPA.
-    - move=> tP tP' tQ' /= [<- <-]. exists t_emp.
-      rewrite !empSPR. split; reflexivity.
-    - move=> tP tP' tQ' /= [<- <-]. exists t_emp.
-      rewrite !empSPR. split; reflexivity.
+      clear IHt1 IHt2. exists (t_star tR1 tR2) => /=.
+      t_simplify_correct. }
+    { move => /= P t IH tC *.
+      have Hprop := @remove_prop_correct e (simplify tC t).1 P.
+      specialize (IH tC _ _ (prod_eta _ _ _)).
+      edestruct remove_prop; simpl_paths; subst;
+      (specialize (Hprop _ (reflexivity _)) || clear Hprop);
+      t_simplify_correct. }
+    { move=> tP tP' tQ' /= [<- <-]. exists t_emp.
+      rewrite !empSPR. split; reflexivity. }
+    { move=> tP tP' tQ' /= [<- <-]. exists t_emp.
+      rewrite !empSPR. split; reflexivity. }
   Qed.
 
   (* Weaker version of correctness theorem. *)
-  Corollary simplify_sufficient e tP tQ tP' tQ' :
-    simplify tP tQ = (tP', tQ') ->
-    eval e tP' |-- eval e tQ'  ->  eval e tP |-- eval e tQ.
+  Corollary simplify_sufficient e tH tC tH' tC' :
+    simplify tC tH = (tC', tH') ->
+    eval e tH' |-- eval e tC'  ->  eval e tH |-- eval e tC.
   Proof.
     move=> Heq H. have [tR [H1 H2]] := simplify_correct e Heq.
-    rewrite ->H1, <-H2. cancel2.
+    rewrite ->H1, ->H2. by f_cancel.
   Qed.
 
-  (* remove emp *)
+  (* remove emp, pull false *)
   Fixpoint clean t :=
     match t with
     | t_star t1 t2 =>
@@ -489,21 +647,81 @@ Module Solving.
         | t', t_emp => t'
         | _, _ => t_star t1' t2'
         end
+    | t_propand P t' =>
+        let t'' := clean t' in
+        match t'' with
+          | t_false => t_false
+          | _ => t_propand P t''
+        end
     | _ => t
     end.
 
   Lemma clean_correct e t : eval e (clean t) -|- eval e t.
   Proof.
-    induction t; try reflexivity; []. rewrite /=.
-    destruct (clean t1); destruct (clean t2); rewrite -IHt1 -IHt2;
+    induction t; try reflexivity.
+    { rewrite /=.
+      destruct (clean t1); destruct (clean t2); rewrite -IHt1 -IHt2;
       try rewrite empSPL; try rewrite empSPR;
-      try rewrite sepSP_falseL; try rewrite sepSP_falseR; reflexivity.
+      try rewrite sepSP_falseL; try rewrite sepSP_falseR; reflexivity. }
+    { simpl; destruct (clean t); simpl in *; rewrite <- IHt; try reflexivity.
+      split; do ?[ reflexivity
+                 | apply lfalseL
+                 | apply lpropandL ]. }
   Qed.
 
-  Lemma do_simplify e tP tQ tP' tQ':
-    simplify tP tQ = (tP', tQ') ->
-    eval e (clean tP') |-- eval e (clean tQ')  ->  eval e tP |-- eval e tQ.
-  Proof. rewrite !clean_correct. apply simplify_sufficient. Qed.
+  (** bring lpropand to the top *)
+  (** I'm lazy, so I'll just count how many t_propands there are, and give the procedure that much fuel *)
+  Definition addn' := Eval lazy in addn.
+  Fixpoint count_t_propand t :=
+    match t with
+      | t_star t1 t2 => addn' (count_t_propand t1) (count_t_propand t2)
+      | t_propand _ t' => (count_t_propand t').+1
+      | _ => 0
+    end.
+
+  Fixpoint pull1_t_propand t :=
+    match t with
+      | t_star t1 t2
+        => let t1' := pull1_t_propand t1 in
+           let t2' := pull1_t_propand t2 in
+           match t1', t2' with
+             | t_propand P1 t1'', t_propand P2 t2'' => t_propand P1 (t_propand P2 (t_star t1'' t2''))
+             | t_propand P t1'', t2'' => t_propand P (t_star t1'' t2'')
+             | t1'', t_propand P t2'' => t_propand P (t_star t1'' t2'')
+             | t1'', t2'' => t_star t1'' t2''
+           end
+      | t_propand P t' => t_propand P (pull1_t_propand t')
+      | _ => t
+    end.
+
+  Fixpoint rep {T} (f : T -> T) x n :=
+    if n is n.+1 then f (rep f x n) else x.
+
+  Definition pull_t_propand t := rep pull1_t_propand t (count_t_propand t).
+
+  Lemma pull1_t_propand_correct e t : eval e (pull1_t_propand t) -|- eval e t.
+  Proof.
+    induction t; try reflexivity;
+    simpl; do !hyp_rewrite <- *; clear; try reflexivity.
+    do 2 edestruct pull1_t_propand;
+      do ![ reflexivity
+          | progress setoid_rewrite <- bilpropandL
+          | progress setoid_rewrite <- bilpropandR ].
+  Qed.
+
+  Lemma pull_t_propand_correct e t : eval e (pull_t_propand t) -|- eval e t.
+  Proof.
+    unfold pull_t_propand.
+    generalize (count_t_propand t) => n.
+    move: t.
+    induction n => * //=.
+    by rewrite -> pull1_t_propand_correct.
+  Qed.
+
+  Lemma do_simplify e tH tC tH' tC':
+    simplify tC tH = (tC', tH') ->
+    eval e (clean (pull_t_propand tH')) |-- eval e (clean (pull_t_propand tC'))  ->  eval e tH |-- eval e tC.
+  Proof. rewrite !clean_correct !pull_t_propand_correct. apply simplify_sufficient. Qed.
 
   (* If speed is an issue at some point, we could make rquote take two
      environments: one to insert into and one to lookup in. Our decision
@@ -511,20 +729,30 @@ Module Solving.
      in common between left and right.
 
      We first try to do unification up to syntax, and try again after we've simpled *)
-  Ltac ssimpl_with doUnify :=
+  Ltac pre_ssimpl_with doUnify :=
     first [ syntax_unify_reflexivity
           | match goal with
               | [ |- ?P |-- ?Q ] =>
-                lquote ((0, [::]) : env) P ltac:(fun e tP =>
+                lquote ((0, [::], [::]) : env) P ltac:(fun e tP =>
                   rquote doUnify e Q ltac:(fun e tQ =>
                     eapply (@do_simplify e tP tQ);
                     [ cbv; reflexivity
-                    | cbv [eval lookup eqn' clean]
+                    | cbv [eval spred_lookup prop_lookup eqn' clean pull_t_propand pull1_t_propand rep count_t_propand addn']
                     ]
                   )
                 )
             end;
             try syntax_unify_reflexivity ].
+
+  (** After we're done, we want to move the things involving
+      [lpropand] in the hypothesis list into the Coq context.  They're
+      all at the top, so we can just apply [lpropandL] repeatedly. *)
+  Ltac post_ssimpl :=
+    repeat match goal with
+             | [ |- _ /\\ _ |-- _ ] => apply lpropandL => *
+           end.
+
+  Ltac ssimpl_with doUnify := pre_ssimpl_with doUnify; post_ssimpl.
 
   Ltac ssimpl := ssimpl_with cheap_unify.
 
@@ -533,21 +761,21 @@ Module Solving.
   Proof. move=> P Q. eexists. ssimpl. done. Qed.
 
   (* TODO: probably subsumed by do_simplify, but this should be faster *)
-  Lemma solve_uc e tP tQ:
-    if remove tP tQ is Some _
-    then eval e tP |-- eval e tQ ** ltrue
+  Lemma solve_uc e tH tC:
+    if remove tH tC is Some _
+    then eval e tH |-- eval e tC ** ltrue
     else True.
   Proof.
-    move Hresult: (remove tP tQ) => result.
+    move Hresult: (remove tH tC) => result.
     destruct result; last done.
-    have Hcorrect := remove_correct Hresult.
-    etransitivity; [apply Hcorrect|]. cancel2.
+    have Hcorrect := remove_correct e Hresult.
+    rewrite -> Hcorrect. by f_cancel.
   Qed.
 
   Ltac solve_uc :=
     match goal with
     |- ?P |-- ?Q ** ltrue =>
-        lquote ((0, [::]) : env) P ltac:(fun e tP =>
+        lquote ((0, [::], [::]) : env) P ltac:(fun e tP =>
           rquote cheap_unify e Q ltac:(fun e tQ =>
             apply (@solve_uc e tP tQ)
           )
