src/charge_lemmas.v
@@ -1,0 +1,29 @@
+(** * Various tactics for dealing with charge logics and separation logics. *)
+Require Import Ssreflect.ssreflect Ssreflect.ssrbool Ssreflect.ssrnat Ssreflect.eqtype Ssreflect.seq Ssreflect.fintype Ssreflect.tuple.
+Require Import x86proved.charge.ilogic x86proved.charge.sepalg x86proved.charge.bilogic x86proved.charge.later x86proved.charge.csetoid.
+Require Import Coq.Setoids.Setoid.
+
+Set Implicit Arguments.
+Unset Strict Implicit.
+Import Prenex Implicits.
+Generalizable All Variables.
+
+(** TODO(t-jagro): Figure out if this already exists somewhere *)
+Lemma lentails_def1  `{@ILogic Frm ILOps'} P Q (H' : forall C, C |-- P -> C |-- Q) : P |-- Q.
+Proof.
+  rewrite <- H'; reflexivity.
+Qed.
+
+Lemma bilpropandR {Frm BILO ILO} `{@BILogic Frm ILO BILO, @ILogic Frm ILO} A (B C : Frm) : A /\\ (B ** C) -|- B ** (A /\\ C).
+Proof.
+  unfold lpropand.
+  split; do [ by rewrite <- bilexistsscL
+            | by rewrite <- bilexistsscR ].
+Qed.
+
+Lemma bilpropandL {Frm BILO ILO} `{@BILogic Frm ILO BILO, @ILogic Frm ILO} A (B C : Frm) : A /\\ (B ** C) -|- (A /\\ B) ** C.
+Proof.
+  unfold lpropand.
+  setoid_rewrite -> sepSPC.
+  apply: bilpropandR.
+Qed.
